[minor] Create new Encodable class.
Factor out encoding as integers from the ConcreteLattice class, in
preparation for the more general notion of label implementation.

pico-ifc-coq/basic_machines/CLattices.v
@@ -1,10 +1,9 @@
-(* A [ConcreteLattice] is a way of encoding some abstract lattice, as
-defined in [Lattices.v], in terms of integers. This is used in the
-fault handler of the concrete machine to interpret the plain integer
-tags as ifc-labels.
+(* A [ConcreteLattice] is a way of computing over the elements of some
+encodable lattice, as defined in [Encodable.v] and [Lattices.v]. This
+is used in the fault handler of the concrete machine to interpret the
+plain integer tags as ifc-labels.
 
-The encoding comprises two conversion functions, [labToZ] and
-[ZToLab], and the implementation of three lattice primitives in
+This comprises the implementation of three lattice primitives in
 machine code, [genBot], [genJoin] and [genFlows]. We also define the
 notion of a correct lattice encoding, [WfConcreteLattice], which will
 be needed when proving the correctness of the fault handler.*)
@@ -20,60 +19,40 @@ Require Import Concrete.
 Require Import CodeGen.
 Require Import CodeTriples. 
 Require Import CodeSpecs.
+Require Import Encodable.
 
 Local Open Scope Z_scope. 
 
-(* A [ConcreteLattice] specifies how to encode some type [T] in terms
-of integers. The last three methods, [genBot], [genJoin], and
-[genFlows], are pieces of code that should implement the three lattice
-methods [bot], [join] and [flows], operating on integers encoding
-elements of [T]. Notice that we don't place any correctness
-assumptions on these operations; these requirements are laid out in
-the [WfConcreteLattice] class, given later. *)
+(* The methods of [ConcreteLattice], are pieces of code that should
+implement the three lattice methods [bot], [join] and [flows],
+operating on integers encoding elements of [T]. Notice that we don't
+place any correctness assumptions on these operations; these
+requirements are laid out in the [WfConcreteLattice] class, given
+later. *)
 
 Class ConcreteLattice (T: Type) :=
-{ labToZ :  T -> Z
-; ZToLab :  Z -> T
-; genBot : list Instr
-; genJoin : list Instr 
+{ genBot : list Instr
+; genJoin : list Instr
 ; genFlows : list Instr
 }.
 
-(* As an example of a lattice encoding, we can encode the simple
-two-point lattice [Lab] by mapping 0 to [L] and any other integer to
-[H]. Thus, [Lab] is encoded in integers just like the [bool] type. The
-operations are simple boolean operations as defined in [CodeGen.v]. *)
+(* As an example, we can implement the simple H/L lattice using the
+implementation of the corresponding boolean operations defined in
+[CodeGen.v] *)
 
 Instance TMUHL : ConcreteLattice Lab :=
 {
-  labToZ l :=
-    match l with
-      | L => boolToZ false
-      | H => boolToZ true
-    end
- 
-  ;ZToLab z :=
-    match z with
-      | 0 => L
-      | _ => H
-    end
-
-  ;genBot := genFalse
-
+  genBot := genFalse
   ;genJoin := genOr
-
   ;genFlows := genImpl
 }.
 
-(* We now define what it means for a lattice encoding to be
-correct. The first requirement, [ZToLab_labToZ_id], says that decoding
-an encoded label gives back the original label. The other three are
-Hoare triples (as defined in [CodeSpecs.v]) specifying that each piece
-of code in [ConcreteLattice] computes exactly what we expect. *)
+(* In order for a lattice implementation to be correct, each piece of
+code in [ConcreteLattice] must compute exactly what we expect. We
+specify that with the Hoare triples defined in [CodeTriples.v]. *)
 
-Class WfConcreteLattice (T: Type) (L : JoinSemiLattice T) (CL: ConcreteLattice T) :=
-{ ZToLab_labToZ_id: forall l, l = ZToLab (labToZ l)
-; genBot_spec: forall Q,
+Class WfConcreteLattice (T: Type) (L : JoinSemiLattice T) (CL: ConcreteLattice T) (E : Encodable T) :=
+{ genBot_spec: forall Q,
    HT genBot
       (fun m s => Q m ((labToZ bot,handlerTag):::s))
       Q
@@ -91,17 +70,8 @@ Class WfConcreteLattice (T: Type) (L : JoinSemiLattice T) (CL: ConcreteLattice T
                                        (labToZ l', handlerTag)::: s0 /\
                             Q m ((boolToZ (flows l l'), handlerTag) ::: s0))
        Q
-       
-}.
 
-Lemma labToZ_inj: forall {L J C} {W: WfConcreteLattice L J C} (l1 l2: L),
-  labToZ l1 = labToZ l2 -> l1 = l2.
-Proof.
-  intros.
-  rewrite (ZToLab_labToZ_id l1).
-  rewrite (ZToLab_labToZ_id l2).
-  apply f_equal; auto.
-Qed.
+}.
 
 (* We can easily show that the encoding of [Lab] above is correct. We
 prove the four required lemmas, and them package them in the [TMUHLwf]
@@ -174,9 +144,8 @@ Proof.
   intuition; eauto.
 Qed.
 
-Instance TMUHLwf : WfConcreteLattice Lab HL TMUHL :=
-{ ZToLab_labToZ_id := ZToLab_labToZ_id_HL
-; genBot_spec := genBot_spec_HL
+Instance TMUHLwf : WfConcreteLattice Lab HL TMUHL EncodableHL :=
+{ genBot_spec := genBot_spec_HL
 ; genJoin_spec := genJoin_spec_HL
 ; genFlows_spec := genFlows_spec_HL
 }.
