pico-ifc-coq/basic_machines/Encodable.v
@@ -1,0 +1,38 @@
+Require Import ZArith.
+Require Import Lattices.
+Require Import CodeGen.
+
+Open Scope Z_scope.
+
+Class Encodable (L : Type) := {
+  labToZ : L -> Z;
+  ZToLab : Z -> L;
+  ZToLab_labToZ_id : forall l, l = ZToLab (labToZ l)
+}.
+
+Program Instance EncodableHL : Encodable Lab := {
+
+  labToZ l :=
+    match l with
+      | L => boolToZ false
+      | H => boolToZ true
+    end
+
+  ;ZToLab z :=
+    match z with
+      | 0 => L
+      | _ => H
+    end
+
+}.
+
+Next Obligation. destruct l; auto. Qed.
+
+Lemma labToZ_inj: forall {L} {W: Encodable L} (l1 l2: L),
+  labToZ l1 = labToZ l2 -> l1 = l2.
+Proof.
+  intros.
+  rewrite (ZToLab_labToZ_id l1).
+  rewrite (ZToLab_labToZ_id l2).
+  apply f_equal; auto.
+Qed.
